


## Level1

$$
d=\frac{1}{2}+\frac{\sqrt{-j}}{2}
$$

### $j=7$

$$
\frac{1}{π}=\frac{\sqrt{15}}{75}\sum_{k=0}^∞\frac{(6 k)!}{(3k)!}\frac{(7⋅9k+8)}{(-1)^k(15^k⋅k!)^3}
$$

### $j=11$

$$
\frac{1}{π}=\sqrt{2}\sum_{k=0}^∞\frac{(6 k)!}{(3k)!}\frac{(11⋅14 k+15) }{(-2)^{15 k+6}(k!)^3}
$$

### $j=19$

$$
\frac{1}{π}=\frac{\sqrt{6}}{3}\sum_{k=0}^∞\frac{(6 k)!}{(3k)!}\frac{(19⋅18 k+25)}{(-2)^{15 k+6} (3^k⋅k!)^3}
$$


### $j=43$

$$
\frac{1}{π}=\frac{\sqrt{15}}{50}\sum_{k=0}^∞\frac{(6 k)!}{(3k)!}\frac{(43⋅126 k+263)}{(-2)^{15 k+6}(30^k⋅k!)^3}
$$

### $j=67$

$$
\frac{1}{π}=\frac{\sqrt{330}}{9075}\sum_{k=0}^∞\frac{(6 k)!}{(3k)!}\frac{(67⋅3906 k+10177) }{(-2)^{15k+6} (165^{k}⋅k!)^3 }
$$

### $j=163$

$$
\frac{1}{π}=\frac{\sqrt{10005}}{66733350}\sum_{k=0}^∞\frac{(6 k)!}{(3k)!}\frac{(163⋅3344418k+13591409)}{(-2)^{15k+6} (20010^k⋅k!)^3}
$$



## Level2

$$
d = \frac{\sqrt{-j}}{2}
$$



### $j=4$

$$
\frac{1}{π}=\frac{2}{9}\sum_{k=0}^∞\frac{(4k)!}{(k!)^4}\frac{(7k+1)}{648^k}
$$

### $j=10$

$$
\frac{1}{π}=\frac{2\sqrt{2}}{9}\sum_{k=0}^∞\frac{(4k)!}{(k!)^4}\frac{(10k+1)}{12^{4k}}
$$

### $j=58$

$$
\frac{1}{π}=\frac{2\sqrt{2}}{9801}\sum_{k=0}^∞\frac{(4k)!}{(k!)^4}\frac{(58⋅455 k+1103)}{396^{4k}}
$$

## Level3

$$
d=\frac{1}{2}+\frac{\sqrt{-j}}{6}
$$

### $j=27$

$$
\frac{1}{π}=\frac{\sqrt{3}}{4}\sum_{k=0}^∞\frac{(2k)!(3k)!}{(k!)^5}\frac{(5k+1)}{(-2^6×3)^k}
$$


### $j=51$

$$
\frac{1}{π}=\frac{\sqrt{3}}{36}\sum_{k=0}^∞\frac{(2k)!(3k)!}{(k!)^5}\frac{(51 k+7)}{(-2^6×3^3)^{k}}
$$

### $j=75$

$$
\frac{1}{π}=\frac{\sqrt{15}}{12}\sum_{k=0}^∞\frac{(2k)!(3k)!}{(k!)^5}\frac{(9 k+1)}{(-2^6×3×5)^k}
$$


### $j=123$

$$
\frac{1}{π}=\frac{\sqrt{3}}{288}\sum_{k=0}^∞\frac{(2k)!(3k)!}{(k!)^5}\frac{(123⋅5 k+53)}{(-2^6×2^6×3^3)^{k}}
$$

### $j=147$

$$
\frac{1}{π}=\frac{\sqrt{7}}{108}\sum_{k=0}^∞\frac{(2k)!(3k)!}{(k!)^5}\frac{(165 k+13)}{\left(-2^6×3^6×7\right)^k}
$$

### $j=267$

$$
\frac{1}{π}=\frac{\sqrt{3}}{4500}\sum_{k=0}^∞\frac{(2k)!(3k)!}{(k!)^5}\frac{(267⋅53k+827)}{(-2^6×3^3×5^3)^{k}}
$$

## Level4

$$
d=\frac{1}{2}+\frac{\sqrt{-j}}{2}
$$

### $j=2$

$$
\frac{1}{π}=\frac{1}{2}\sum_{k=0}^∞(-1)^k\left(\frac{(2 k)!}{(k!)^2}\right)^3\frac{(4 k+1)}{2^{6k}}
$$

### $j=4$

$$
\frac{1}{π}=\frac{\sqrt{2}}{4}\sum_{k=0}^∞(-1)^k\left(\frac{(2 k)!}{(k!)^2}\right)^3\frac{(6 k+1)}{2^{9k}}
$$

## Level5

$$
d=\frac{1}{2}+\frac{\sqrt{-5j}}{10}
$$
