$$
\begin{aligned}
&\sum_{k=0}^∞\frac{8}{(4k+1)(4k+3)}=\frac{0}{1}-π\\
&Δ=3.141592653589793\\
\end{aligned}
$$

$$
\begin{aligned}
&\sum_{k=0}^∞\frac{24}{(4k+1)(4k+2)(4k+4)}=\frac{0}{1}-π\\
&Δ=3.141592653589793\\
\end{aligned}
$$

$$
\begin{aligned}
&\sum_{k=0}^∞\frac{48}{(4k+1)(4k+3)(4k+7)}=π-\frac{2}{3}\\
&Δ=2.4749259869231266\\
\end{aligned}
$$

$$
\begin{aligned}
&\sum_{k=0}^∞\frac{24}{(4k+1)(4k+7)}=\frac{4}{3}-π\\
&Δ=1.80825932025646\\
\end{aligned}
$$

$$
\begin{aligned}
&\sum_{k=0}^∞\frac{48}{(4k+1)(4k+5)(4k+7)}=\frac{14}{3}-π\\
&Δ=1.5250740130768734\\
\end{aligned}
$$

$$
\begin{aligned}
&\sum_{k=0}^∞\frac{120}{(4k+1)(4k+2)(4k+6)(4k+7)}=π-\frac{5}{3}\\
&Δ=1.4749259869231266\\
\end{aligned}
$$

$$
\begin{aligned}
&\sum_{k=0}^∞\frac{16}{(4k+1)(4k+3)(4k+5)}=π-\frac{2}{1}\\
&Δ=1.1415926535897931\\
\end{aligned}
$$

$$
\begin{aligned}
&\sum_{k=0}^∞\frac{8}{(4k+3)(4k+5)}=\frac{4}{1}-π\\
&Δ=0.8584073464102068\\
\end{aligned}
$$

$$
\begin{aligned}
&\sum_{k=0}^∞\frac{48}{(4k+1)(4k+3)(4k+5)(4k+7)}=π-\frac{8}{3}\\
&Δ=0.4749259869231266\\
\end{aligned}
$$

$$
\begin{aligned}
&\sum_{k=0}^∞\frac{16}{(4k+3)(4k+5)(4k+7)}=\frac{10}{3}-π\\
&Δ=0.1917406797435401\\
\end{aligned}
$$

$$
\begin{aligned}
&\sum_{k=0}^∞\frac{24}{(4k+4)(4k+6)(4k+7)}=\frac{10}{3}-π\\
&Δ=0.1917406797435401\\
\end{aligned}
$$

$$
\begin{aligned}
&\sum_{k=0}^∞\frac{240}{(4k+1)(4k+2)(4k+3)(4k+5)(4k+6)(4k+7)}=\frac{10}{3}-π\\
&Δ=0.1917406797435401\\
\end{aligned}
$$

$$
\begin{aligned}
&\sum_{k=0}^∞\frac{24}{(4k+2)(4k+3)(4k+5)(4k+6)}=π-\frac{3}{1}\\
&Δ=0.14159265358979323\\
\end{aligned}
$$

$$
\begin{aligned}
&\sum_{k=0}^∞\frac{24}{(4k+4)(4k+5)(4k+7)(4k+8)}=\frac{19}{6}-π\\
&Δ=0.025074013076873427\\
\end{aligned}
$$

